\subsection{Arithmetic Expressions}
Old
\begin{table}[H]
    \centering
    \begin{longtable}[c] { r c }
        [PLUS-1] & \( \dfrac{a_1 \Rightarrow a^{'}_{1}}{a_1 + a_2 \Rightarrow a^{'}_{1} + a_2} \) \\
        
        [PLUS-2] & \( \dfrac{a_2 \Rightarrow a^{'}_{2}}{v_1 + a_2 \Rightarrow v_1 + a^{'}_{2}} \) \\
        
        [PLUS-3] & \(z_1 + z_2 \Rightarrow z \text{ where } z = v_1 + v_2\) \\
    \end{longtable}
    \caption{Small-step semantics for arithmetic plus expressions}\label{tab:sss_aud}
\end{table}
New
\begin{table}[H]
    \centering
    \begin{longtable}[c] { r c }
        [PLUS-1] & \( \dfrac{ env_v,sto \vdash a_1 \rightarrow_a a^{'}_{1}}{env_v,sto \vdash a_1 + a_2 \rightarrow a^{'}_{1} + a_2} \) \\
        
        [PLUS-2] & \( \dfrac{ env_v,sto \vdash a_2 \rightarrow_a a^{'}_{2}}{env_v,sto \vdash v_1 + a_2 \rightarrow a_{1} + a_2{'}} \) \\
        
        [PLUS-3] & \(v_1 + v_2 \Rightarrow v \text{ where } v = v_1 + v_2\) \\
    \end{longtable}
    \caption{Small-step semantics for arithmetic plus expressions}\label{tab:sss_aud}
\end{table}
\begin{table}[H]
    \centering
    \begin{longtable}[c] { r c }
        
        [MINUS-1] & \( \dfrac{a_1 \Rightarrow a^{'}_{1}}{a_1 - a_2 \Rightarrow a^{'}_{1} - a_2} \) \\
        
        [MINUS-2] & \( \dfrac{a_2 \Rightarrow a^{'}_{2}}{v_1 - a_2 \Rightarrow v_1 - a^{'}_{2}} \) \\
        
        [MINUS-3] & \(v_1 - v_2 \Rightarrow z \text{ where } z = v_1 - v_2\) \\
        
        
    \end{longtable}
    \caption{Small-step semantics for arithmetic minus expressions}\label{tab:sss_aud}
\end{table}
\begin{table}[H]
    \centering
    \begin{longtable}[c] { r c }
        
        [MULT-1] & \( \dfrac{a_1 \Rightarrow a^{'}_{1}}{a_1 * a_2 \Rightarrow a^{'}_{1} * a_2} \) \\
        
        [MULT-2] & \( \dfrac{a_2 \Rightarrow a^{'}_{2}}{v_1 * a_2 \Rightarrow v_1 * a^{'}_{2}} \) \\
        
        [MULT-3] & \(v_1 * v_2 \Rightarrow z \text{ where } z = v_1 \cdot v_2\) \\
        
    \end{longtable}
    \caption{Small-step semantics for arithmetic multiplicative expressions}\label{tab:sss_aud}
\end{table}
\begin{table}[H]
    \centering
    \begin{longtable}[c] { r c }
        
        [DIV-1] & \( \dfrac{a_1 \Rightarrow a^{'}_{1}}{a_1 / a_2 \Rightarrow a^{'}_{1} / a_2} \) \\
        
        [DIV-2] & \( \dfrac{a_2 \Rightarrow a^{'}_{2}}{v_1 / a_2 \Rightarrow v_1 / a^{'}_{2}} \) \\
        
        [DIV-3] & \(v_1 / v_2 \Rightarrow z \text{ where } z = \lfloor\frac{v_1} {v_2}\rfloor\) \\
        
    \end{longtable}
    \caption{Small-step semantics for arithmetic expressions}\label{tab:sss_aud}
\end{table}
        \begin{table}[H]
    \centering
    \begin{longtable}[c] { r c }
        [PARENT-1] & \( \dfrac{a_1 \Rightarrow a^{'}_{1}}{(a_1) \Rightarrow (a^{'}_{1})} \) \\
        
        [PARENT-2] & \( (z) \Rightarrow z \) \\
        
    \end{longtable}
    \caption{Small-step semantics for arithmetic parenthesis expressions}\label{tab:sss_aud}
\end{table}
\begin{table}[H]
    \centering
    \begin{longtable}[c] { r c }
        
        [NEG-1] & \( \dfrac{a_1 \Rightarrow a^{'}_{1}}{-a_1 \Rightarrow -a^{'}_{1}} \) \\
        
        [NEG-2] & \( -v_1 \Rightarrow z \text{ where } z = -v_1 \)\\
        
    \end{longtable}
    \caption{Small-step semantics for arithmetic negation expressions}\label{tab:sss_aud}
\end{table}
\begin{table}[H]
    \centering
    \begin{longtable}[c] { r c }
        
        [INT-1] & \( n \Rightarrow z \text{ if } \mathbb{Z}[[n]] = z \) \\
        
        [INT-2] & \( v \Rightarrow z \text{ if } v \in \mathbb{Z} \)\\
        
    \end{longtable}
    \caption{Small-step semantics for arithmetic integer expressions}\label{tab:sss_aud}
\end{table}